src/scratch.lean
@@ -4,12 +4,4 @@ open robot
 namespace scratch1
 open tactic
 
-    run_cmd do
-        mv ← mk_mvar,
-        E ← to_expr ```(%%mv + %%mv),
-        trace E,
-        let E₂ := expr.abstract E mv,
-        trace E₂,
-        skip
-
 end scratch1
